src/cbor/pulse/CBOR.Pulse.API.Det.Dummy.fsti
@@ -7,3 +7,9 @@ val dummy_cbor_det_t (_: unit) : T.cbor_det_t
 
 inline_for_extraction
 val dummy_cbor_det_array_append_cell (_: unit) : T.cbor_det_array_append_cell_t
+
+inline_for_extraction
+val dummy_cbor_det_map_entry_insert_cell (_: unit) : T.cbor_det_map_entry_insert_cell_t
+
+inline_for_extraction
+val dummy_cbor_det_map_entry (_: unit) : T.cbor_det_map_entry_t
